\documentclass{article}
\usepackage{amsmath}
\usepackage{amssymb}
\usepackage[T1,T2A]{fontenc}
\usepackage[utf8]{inputenc}
\usepackage[bulgarian]{babel}
\usepackage[normalem]{ulem}
\newcommand{\stkout}[1]{\ifmmode\text{\sout{\ensuremath{#1}}}\else\sout{#1}\fi}

\begin{document}
    \pagenumbering{gobble}
    \begin{math}
        \\
        \text{а)} \lim_{n \to \infty} \frac{2n^3 + 3n + 5}{-3n^3 + 4n + 7}\\
        \\
        \lim_{n \to \infty} \frac{2n^3 + 3n + 5}{-3n^3 + 4n + 7}\\
        \\
        \lim_{n \to \infty} \frac{\stkout{n^3}(2 + \frac{3}{n^2} + \frac{5}{n^3})}{\stkout{n^3}(-3 + \frac{4}{n^2} + \frac{7}{n^3})}\\
        \\
        \lim_{n \to \infty} \frac{2 + \frac{3}{n^2} + \frac{5}{n^3}}{-3 + \frac{4}{n^2} + \frac{7}{n^3}}\\
        \\
        \lim_{n \to \infty} \frac{2 + 3\frac{1}{n}\frac{1}{n} + 5\frac{1}{n}\frac{1}{n}\frac{1}{n}}{-3 + 4\frac{1}{n}\frac{1}{n} + 7\frac{1}{n}\frac{1}{n}\frac{1}{n}}\\
        \\
        \frac{1}{n} \to 0 \implies \lim_{n \to \infty} \frac{2 + 3\times0 + 5\times0}{-3 + 4\times0 + 7\times0}\\
        \\
        \implies \lim_{n \to \infty} \frac{2n^3 + 3n + 5}{-3n^3 + 4n + 7} = \frac{-2}{3}\\
        \\
        \\
        \text{в)} \lim_{n \to \infty} \frac{n}{\sqrt{n^4 + 3n^2 + 4} - \sqrt{n^4 - n^3 + 1}}\\
        \\
        \lim_{n \to \infty} \frac{n}{\sqrt{n^4 + 3n^2 + 4} - \sqrt{n^4 - n^3 + 1}}\\
        \\
        \lim_{n \to \infty} \frac{n}{\sqrt{n^4 + 3n^2 + 4} - \sqrt{n^4 - n^3 + 1}}\frac{\sqrt{n^4 + 3n^2 + 4} + \sqrt{n^4 - n^3 + 1}}{\sqrt{n^4 + 3n^2 + 4} + \sqrt{n^4 - n^3 + 1}}\\
        \\
        \lim_{n \to \infty} \frac{n(\sqrt{n^4 + 3n^2 + 4} + \sqrt{n^4 - n^3 + 1})}{(\sqrt{n^4 + 3n^2 + 4})^2 - (\sqrt{n^4 - n^3 + 1})^2}\\
        \\
        \lim_{n \to \infty} \frac{n\sqrt{n^4}(\sqrt{1 + \frac{3}{n^2} + \frac{4}{n^4}} + \sqrt{1 - \frac{1}{n} + \frac{1}{n^4}})}{(n^4 + 3n^2 + 4) - (n^4 - n^3 + 1)}\\
        \\
        \lim_{n \to \infty} \frac{n^3(\sqrt{1 + \frac{3}{n^2} + \frac{4}{n^4}} + \sqrt{1 - \frac{1}{n} + \frac{1}{n^4}})}{n^3 + 3n^2 + 3}\\
        \\
        \lim_{n \to \infty} \frac{\stkout{n^3}(\sqrt{1 + \frac{3}{n^2} + \frac{4}{n^4}} + \sqrt{1 - \frac{1}{n} + \frac{1}{n^4}})}{\stkout{n^3}(1 + \frac{3}{n} + \frac{3}{n^3})}\\
        \\
        \lim_{n \to \infty} \frac{\sqrt{1 + 3\frac{1}{n}\frac{1}{n} + 4\frac{1}{n}\frac{1}{n}\frac{1}{n}\frac{1}{n}} + \sqrt{1 - \frac{1}{n} + \frac{1}{n}\frac{1}{n}\frac{1}{n}\frac{1}{n}}}{1 + 3\frac{1}{n} + 3\frac{1}{n}\frac{1}{n}\frac{1}{n}}\\
        \\
        \frac{1}{n} \to 0 \implies \lim_{n \to \infty} \frac{\sqrt{1 + 3\times0 + 4\times0} + \sqrt{1 - 0 + 0}}{1 + 3\times0 + 3\times0}\\
        \\
        \implies \lim_{n \to \infty} \frac{n}{\sqrt{n^4 + 3n^2 + 4} - \sqrt{n^4 - n^3 + 1}} = 2\\
    \end{math}
\end{document}