\documentclass{article}
\usepackage{amsmath}
\usepackage{amssymb}
\usepackage[T1,T2A]{fontenc}
\usepackage[utf8]{inputenc}
\usepackage[bulgarian]{babel}
\usepackage[normalem]{ulem}
\newcommand{\stkout}[1]{\ifmmode\text{\sout{\ensuremath{#1}}}\else\sout{#1}\fi}

\makeatletter
\renewcommand*\env@matrix[1][*\c@MaxMatrixCols c]{%
  \hskip -\arraycolsep
  \let\@ifnextchar\new@ifnextchar
  \array{#1}}
\makeatother

\begin{document}
    \pagenumbering{gobble}
    \begin{math}
        \\
        a = \alpha_1 x ^ 3 + \alpha_2 x ^ 2 + \alpha_3 x ^ 1 + \alpha_4\\
        b = \beta_1 x ^ 3 + \beta_2 x ^ 2 + \beta_3 x ^ 1 + \beta_4\\
        c = \gamma_1 x ^ 3 + \gamma_2 x ^ 2 + \gamma_3 x ^ 1 + \gamma_4\\
        a' = \alpha_1' x ^ 3 + \alpha_2' x ^ 2 + \alpha_3' x ^ 1 + \alpha_4'\\
        a, b, c, a' \in \mathbb{V}\\
        \lambda, \mu, \alpha_1, \alpha_2, \alpha_3, \alpha_4, \beta_1, \beta_2, \beta_3, \beta_4, \gamma_1, \gamma_2, \gamma_3, \gamma_4, \alpha_1', \alpha_2', \alpha_3', \alpha_4' \in \mathbb{F}\\
        \\
        1.\quad(a + b) + c = a + (b + c)\\
        \\
        (a + b) = (\alpha_1 x ^ 3 + \alpha_2 x ^ 2 + \alpha_3 x ^ 1 + \alpha_4)
        + (\beta_1 x ^ 3 + \beta_2 x ^ 2 + \beta_3 x ^ 1 + \beta_4)
        = (\alpha_1 + \beta_1) x ^ 3 + (\alpha_2 + \beta_2) x ^ 2
        + (\alpha_3 + \beta_3) x ^ 1 + (\alpha_4 + \beta_4)\\
        \\
        (a + b) + c = (\alpha_1 + \beta_1) x ^ 3 + (\alpha_2 + \beta_2) x ^ 2 + (\alpha_3 + \beta_3) x ^ 1 + (\alpha_4 + \beta_4)
        + (\gamma_1 x ^ 3 + \gamma_2 x ^ 2 + \gamma_3 x ^ 1 + \gamma_4)
        = (\alpha_1 + \beta_1 + \gamma) x ^ 3 + (\alpha_2 + \beta_2 + \gamma) x ^ 2 + (\alpha_3 + \beta_3 + \gamma) x ^ 1 + (\alpha_4 + \beta_4 + \gamma)\\
        \\
        (b + c) = (\beta_1 x ^ 3 + \beta_2 x ^ 2 + \beta_3 x ^ 1 + \beta_4) + (\gamma_1 x ^ 3 + \gamma_2 x ^ 2 + \gamma_3 x ^ 1 + \gamma_4)
        = (\beta_1 + \gamma_1) x ^ 3 + (\beta_2 + \gamma_2) x ^ 2 + (\beta_3 + \gamma_3) x ^ 1 + (\beta_4 + \gamma_4)\\
        \\
        a + (b + c) = (\alpha_1 x ^ 3 + \alpha_2 x ^ 2 + \alpha_3 x ^ 1 + \alpha_4)
        + (\beta_1 + \gamma_1) x ^ 3 + (\beta_2 + \gamma_2) x ^ 2 + (\beta_3 + \gamma_3) x ^ 1 + (\beta_4 + \gamma_4)
        = (\alpha_1 + \beta_1 + \gamma) x ^ 3 + (\alpha_2 + \beta_2 + \gamma) x ^ 2 + (\alpha_3 + \beta_3 + \gamma) x ^ 1 + (\alpha_4 + \beta_4 + \gamma)\\
        \\
        \implies (a + b) + c = a + (b + c) = a + b + c\\
        \\
        2.\quad a + b = b + a\\
        \\
        (a + b) = (\alpha_1 x ^ 3 + \alpha_2 x ^ 2 + \alpha_3 x ^ 1 + \alpha_4)
        + (\beta_1 x ^ 3 + \beta_2 x ^ 2 + \beta_3 x ^ 1 + \beta_4)
        = (\alpha_1 + \beta_1) x ^ 3 + (\alpha_2 + \beta_2) x ^ 2
        + (\alpha_3 + \beta_3) x ^ 1 + (\alpha_4 + \beta_4)\\
        \\
        (b + a) = (\beta_1 x ^ 3 + \beta_2 x ^ 2 + \beta_3 x ^ 1 + \beta_4)
        + (\alpha_1 x ^ 3 + \alpha_2 x ^ 2 + \alpha_3 x ^ 1 + \alpha_4)
        = (\alpha_1 + \beta_1) x ^ 3 + (\alpha_2 + \beta_2) x ^ 2
        + (\alpha_3 + \beta_3) x ^ 1 + (\alpha_4 + \beta_4)\\
        \\
        \implies a + b = b + a\\
        \\
        3.\quad a + 0 = a\\
        \\
        a + 0 = (\alpha_1 x ^ 3 + \alpha_2 x ^ 2 + \alpha_3 x ^ 1 + \alpha_4) + (0 x ^ 3 + 0 x ^ 2 + 0 x ^ 1 + 0)
        = (\alpha_1 + 0) x ^ 3 + (\alpha_2 + 0) x ^ 2
        + (\alpha_3 + 0) x ^ 1 + (\alpha_4 + 0)
        = \alpha_1 x ^ 3 + \alpha_2 x ^ 2 + \alpha_3 x ^ 1 + \alpha_4\\
        \\
        \implies a + 0 = a\\
        \\
        4.\quad \exists\,a': a + a' = 0\\
        \\
        a + a' = 0\\
        (\alpha_1 x ^ 3 + \alpha_2 x ^ 2 + \alpha_3 x ^ 1 + \alpha_4) + (\alpha_1' x ^ 3 + \alpha_2' x ^ 2 + \alpha_3' x ^ 1 + \alpha_4') = (0 x ^ 3 + 0 x ^ 2 + 0 x ^ 1 = 0)\\
        (\alpha_1 + \alpha_1') x ^ 3 + (\alpha_2 + \alpha_2') x ^ 2 + (\alpha_3 + \alpha_3') x ^ 1 + (\alpha_4 + \alpha_4') = (0 x ^ 3 + 0 x ^ 2 + 0 x ^ 1 = 0)\\
        \\
        \equiv\quad
        \begin{matrix}[|ccccc]
            \alpha_1' & + & \alpha_1' & = & 0\\
            \alpha_2 & + & \alpha_2' & = & 0\\
            \alpha_3 & + & \alpha_3' & = & 0\\
            \alpha_4 & + & \alpha_4' & = & 0\\
        \end{matrix}
        \quad\to\quad
        \begin{matrix}[|ccc]
            \alpha_1' & = & -\alpha_1\\
            \alpha_2' & = & -\alpha_2\\
            \alpha_3' & = & -\alpha_3\\
            \alpha_4' & = & -\alpha_4\\
        \end{matrix}\\
        \\
        \\
        \implies a' = -\alpha_1 x ^ 3 + -\alpha_2 x ^ 2 + -\alpha_3 x ^ 1 + -\alpha_4 = -(\alpha_1 x ^ 3 + \alpha_2 x ^ 2 + \alpha_3 x ^ 1 + \alpha_4) = -a\\
        \implies \exists\,a': a + a' = 0\\
        \\
        5.\quad 1a = a\\
        \\
        1a = 1(\alpha_1 x ^ 3 + \alpha_2 x ^ 2 + \alpha_3 x ^ 1 + \alpha_4)
        = (1\alpha_1) x ^ 3 + (1\alpha_2) x ^ 2 + (1\alpha_3) x ^ 1 + (1\alpha_4)
        = \alpha_1 x ^ 3 + \alpha_2 x ^ 2 + \alpha_3 x ^ 1 + \alpha_4\\
        \\
        \implies 1a = a\\
        \\
        6.\quad \lambda(a + b) = \lambda a + \lambda b\\
        \\
        \lambda(a + b) = \lambda[(\alpha_1 + \beta_1) x ^ 3 + (\alpha_2 + \beta_2) x ^ 2 + (\alpha_3 + \beta_3) x ^ 1 + (\alpha_4 + \beta_4)]
        = \lambda(\alpha_1 + \beta_1) x ^ 3 + \lambda(\alpha_2 + \beta_2) x ^ 2 + \lambda(\alpha_3 + \beta_3) x ^ 1 + \lambda(\alpha_4 + \beta_4)
        = (\lambda\alpha_1 + \lambda\beta_1) x ^ 3 + (\lambda\alpha_2 + \lambda\beta_2) x ^ 2 + (\lambda\alpha_3 + \lambda\beta_3) x ^ 1 + (\lambda\alpha_4 + \lambda\beta_4)\\
        \\
        \lambda a = \lambda(\alpha_1 x ^ 3 + \alpha_2 x ^ 2 + \alpha_3 x ^ 1 + \alpha_4)
        = \lambda\alpha_1 x ^ 3 + \lambda\alpha_2 x ^ 2 + \lambda\alpha_3 x ^ 1 + \lambda\alpha_4\\
        \\
        \lambda b = \lambda(\beta_1 x ^ 3 + \beta_2 x ^ 2 + \beta_3 x ^ 1 + \beta_4)
        = \lambda\beta_1 x ^ 3 + \lambda\beta_2 x ^ 2 + \lambda\beta_3 x ^ 1 + \lambda\beta_4\\
        \\
        \lambda a + \lambda b = (\lambda\alpha_1 x ^ 3 + \lambda\alpha_2 x ^ 2 + \lambda\alpha_3 x ^ 1 + \lambda\alpha_4) + (\lambda\beta_1 x ^ 3 + \lambda\beta_2 x ^ 2 + \lambda\beta_3 x ^ 1 + \lambda\beta_4)
        = (\lambda\alpha_1 + \lambda\beta_1) x ^ 3 + (\lambda\alpha_2 + \lambda\beta_2) x ^ 2 + (\lambda\alpha_3 + \lambda\beta_3) x ^ 1 + (\lambda\alpha_4 + \lambda\beta_4)\\
        \\
        \implies \lambda(a + b) = \lambda a + \lambda b\\
        \\
        7.\quad (\lambda + \mu)a = \lambda a + \mu a\\
        \\
        (\lambda + \mu)a = (\lambda + \mu)(\alpha_1 x ^ 3 + \alpha_2 x ^ 2 + \alpha_3 x ^ 1 + \alpha_4)
        = [(\lambda + \mu)\alpha_1] x ^ 3 + [(\lambda + \mu)\alpha_2] x ^ 2 + [(\lambda + \mu)\alpha_3] x ^ 1 + [(\lambda + \mu)\alpha_4]
        = (\lambda\alpha_1 + \mu\alpha_1) x ^ 3 + (\lambda\alpha_2 + \mu\alpha_2) x ^ 2 + (\lambda\alpha_3 + \mu\alpha_3) x ^ 1 + (\lambda\alpha_4 + \mu\alpha_4)\\
        \\
        \lambda a = \lambda(\alpha_1 x ^ 3 + \alpha_2 x ^ 2 + \alpha_3 x ^ 1 + \alpha_4)
        = \lambda\alpha_1 x ^ 3 + \lambda\alpha_2 x ^ 2 + \lambda\alpha_3 x ^ 1 + \lambda\alpha_4\\
        \\
        \mu a = \mu(\alpha_1 x ^ 3 + \alpha_2 x ^ 2 + \alpha_3 x ^ 1 + \alpha_4)
        = \mu\alpha_1 x ^ 3 + \mu\alpha_2 x ^ 2 + \mu\alpha_3 x ^ 1 + \mu\alpha_4\\
        \\
        \lambda a + \mu a = (\lambda\alpha_1 x ^ 3 + \lambda\alpha_2 x ^ 2 + \lambda\alpha_3 x ^ 1 + \lambda\alpha_4) + (\mu\alpha_1 x ^ 3 + \mu\alpha_2 x ^ 2 + \mu\alpha_3 x ^ 1 + \mu\alpha_4)
        = (\lambda\alpha_1 + \mu\alpha_1) x ^ 3 + (\lambda\alpha_2 + \mu\alpha_2) x ^ 2 + (\lambda\alpha_3 + \mu\alpha_3) x ^ 1 + (\lambda\alpha_4 + \mu\alpha_4)\\
        \\
        \implies (\lambda + \mu)a = \lambda a + \mu a\\
        \\
        8.\quad \lambda(\mu a) = \lambda \mu a\\
        \\
        \mu a = \mu(\alpha_1 x ^ 3 + \alpha_2 x ^ 2 + \alpha_3 x ^ 1 + \alpha_4)
        = \mu\alpha_1 x ^ 3 + \mu\alpha_2 x ^ 2 + \mu\alpha_3 x ^ 1 + \mu\alpha_4\\
        \\
        \lambda(\mu a) = \lambda(\mu\alpha_1 x ^ 3 + \mu\alpha_2 x ^ 2 + \mu\alpha_3 x ^ 1 + \mu\alpha_4)
        = \lambda(\mu\alpha_1 x ^ 3 + \mu\alpha_2 x ^ 2 + \mu\alpha_3 x ^ 1 + \mu\alpha_4)
        = \lambda\mu\alpha_1 x ^ 3 + \lambda\mu\alpha_2 x ^ 2 + \lambda\mu\alpha_3 x ^ 1 + \lambda\mu\alpha_4)
        = \lambda\mu(\alpha_1 x ^ 3 + \alpha_2 x ^ 2 + \alpha_3 x ^ 1 + \alpha_4) = \lambda\mu a\\
        \\
        \implies \lambda(\mu a) = \lambda \mu a
    \end{math}
\end{document}