\documentclass{article}
\usepackage{amsmath}
\usepackage{amssymb}
\usepackage[T1,T2A]{fontenc}
\usepackage[utf8]{inputenc}
\usepackage[bulgarian]{babel}
\usepackage[normalem]{ulem}
\newcommand{\stkout}[1]{\ifmmode\text{\sout{\ensuremath{#1}}}\else\sout{#1}\fi}

\makeatletter
\renewcommand*\env@matrix[1][*\c@MaxMatrixCols c]{%
  \hskip -\arraycolsep
  \let\@ifnextchar\new@ifnextchar
  \array{#1}}
\makeatother

\renewcommand\thesection{\Roman{section}}

\begin{document}
    \pagenumbering{gobble}
    \begin{math}
        \begin{matrix}
          4x_1 & + & 3x_2 & + & 3x_3 & - & 2x_4 & = & \lambda\\
          -x_1 & - & x_2 & - & x_3 & + & x_4 & = & 2\\
          -19x_1 & - & 19x_2 & - & 20x_3 & + & (11 + \mu)x_4 & = & 6 - 2\lambda\\
          4x_1 & + & 7x_2 & + & 8x_3 & + & x_4 & = & -2
        \end{matrix}\\
        \\
        \\
        \begin{matrix}
          3\\
          ~\\
          -20\\
          8
        \end{matrix}
        \begin{pmatrix}[cccc|c]
            4 & 3 & 3 & -2 &  \lambda\\
            -1  &  -1 &  -1 & 1 & 2\\
            -19 & -19 & -20 & 11 + \mu & 6 - 2\lambda\\
            4 & 7 & 8 & 1 & -2
        \end{pmatrix}\\
        \\
        \\
        \to
        \begin{matrix}
          ~\\
          -1\\
          1\\
          ~
        \end{matrix}
        \begin{pmatrix}[cccc|c]
            1 & 0 & 0 & 1 & \lambda + 6\\
            -1 & -1 & -1 & 1 & 2\\
            1 & 1 & 0 & \mu - 9 & -2\lambda - 34\\
            -4 & -1 & 0 & 9 & 14
        \end{pmatrix}\\
        \\
        \\
        \to
        \begin{matrix}
          ~\\
          -3\\
          3\\
          4
        \end{matrix}
        \begin{pmatrix}[cccc|c]
            1 & 0 & 0 & 1 & \lambda + 6\\
            3 & 0 & -1 & -8 & -12\\
            -3 & 0 & 0 & \mu & -2\lambda - 20\\
            -4 & -1 & 0 & 9 & 14
        \end{pmatrix}\\
        \\
        \\
        \to
        \begin{pmatrix}[cccc|c]
            1 & 0 & 0 & 1 & \lambda + 6\\
            0 & 0 & -1 & -11 & -3\lambda - 30\\
            0 & 0 & 0 & \mu + 3 & \lambda - 2\\
            0 & -1 & 0 & 13 & 4\lambda + 38
        \end{pmatrix}
        \begin{matrix}
          ~\\
          -1\\
          ~\\
          ~
        \end{matrix}\\
        \\
        \\
        \to
        \begin{pmatrix}[cccc|c]
            1 & 0 & 0 & 1 & \lambda + 6\\
            0 & 0 & 1 & 11 & 3\lambda + 30\\
            0 & 0 & 0 & \mu + 3 & \lambda - 2\\
            0 & -1 & 0 & 13 & 4\lambda + 38
        \end{pmatrix}\\
        \\
        \\
        \begin{matrix}[|ccccc]
            x_1 & + & x_4 & = & \lambda + 6\\
            x_3 & + & 11x_4 & = & 3\lambda + 30\\
            ~ & ~ & (\mu + 3)x_4 & = & \lambda - 2\\
            -x_2 & + & 13x_4 & = & 4\lambda + 38
        \end{matrix}
    \end{math}
    \section{\(\mu = -3\)}
    \subsection{\(\lambda = 2\)}
    \begin{math}
        \begin{matrix}[|ccccc]
            x_1 & + & x_4 & = & \lambda + 6\\
            x_3 & + & 11x_4 & = & 3\lambda + 30\\
            ~ & ~ & 0x_4 & = & 0\\
            -x_2 & + & 13x_4 & = & 4\lambda + 38
        \end{matrix}
    \end{math}
    \subsection{\(\lambda \neq 2\)}
    \begin{math}
        \begin{matrix}[|ccccc]
            x_1 & + & x_4 & = & \lambda + 6\\
            x_3 & + & 11x_4 & = & 3\lambda + 30\\
            ~ & ~ & 0x_4 & = & \lambda - 2\\
            -x_2 & + & 13x_4 & = & 4\lambda + 38
        \end{matrix}
    \end{math}
    \section{\(\mu \neq -3\)}
    \subsection{\(\lambda = 2\)}
    \begin{math}
        \begin{matrix}[|ccccc]
            x_1 & + & x_4 & = & \lambda + 6\\
            x_3 & + & 11x_4 & = & 3\lambda + 30\\
            ~ & ~ & (\mu + 3)x_4 & = & 0\\
            -x_2 & + & 13x_4 & = & 4\lambda + 38
        \end{matrix}\\
        \\
        \\
        \to\quad
        \begin{matrix}[|ccc]
            x_1 & = & \lambda + 6\\
            x_3 & = & 3\lambda + 30\\
            x_4 & = & 0\\
            x_2 & = & -4\lambda - 38
        \end{matrix}
    \end{math}
    \subsection{\(\lambda \neq 2\)}
    \begin{math}
        \begin{matrix}[|ccccc]
            x_1 & + & x_4 & = & \lambda + 6\\
            x_3 & + & 11x_4 & = & 3\lambda + 30\\
            ~ & ~ & (\mu + 3)x_4 & = & \lambda - 2\\
            -x_2 & + & 13x_4 & = & 4\lambda + 38
        \end{matrix}\\
        \\
        \\
        \to\quad
        \begin{matrix}[|ccccc]
            x_1 & + & \frac{\lambda - 2}{\mu + 3} & = & \lambda + 6\\
            x_3 & + & 11\frac{\lambda - 2}{\mu + 3} & = & 3\lambda + 30\\
            ~ & ~ & x_4 & = & \frac{\lambda - 2}{\mu + 3}\\
            -x_2 & + & 13\frac{\lambda - 2}{\mu + 3} & = & 4\lambda + 38
        \end{matrix}\\
        \\
        \\
        \to\quad
        \begin{matrix}[|ccc]
            x_1 & = & \frac{(\lambda + 6)(\mu + 3) - (\lambda - 2)}{\mu + 3}\\
            x_3 & + & \frac{(3\lambda + 30)(11\mu + 33) - (11\lambda - 22)}{11\mu + 33}\\
            x_4 & = & \frac{\lambda - 2}{\mu + 3}\\
            x_2 & = & -\frac{(4\lambda + 38)(13\mu + 39) - (13\lambda - 26)}{13\mu + 39}
        \end{matrix}\\
        \\
        \\
        \to\quad
        \begin{matrix}[|ccc]
            x_1 & = & \frac{\lambda\mu + 2\lambda + 6\mu + 20}{\mu + 3}\\
            x_3 & = & \frac{33\mu + 88\lambda + 330\mu + 1012}{11\mu + 33}\\
            x_4 & = & \frac{\lambda - 2}{\mu + 3}\\
            x_2 & = & -\frac{52\lambda\mu + 143\lambda + 494\mu + 1498}{13\mu + 39}
        \end{matrix}
    \end{math}
\end{document}