\documentclass{article}
\usepackage{amsmath}
\usepackage{amssymb}
\usepackage[T1,T2A]{fontenc}
\usepackage[utf8]{inputenc}
\usepackage[bulgarian]{babel}
\usepackage[normalem]{ulem}
\newcommand{\stkout}[1]{\ifmmode\text{\sout{\ensuremath{#1}}}\else\sout{#1}\fi}

\begin{document}
    \pagenumbering{gobble}
    \begin{align*}
        \omega_0, \omega_1, \dots, \omega_{71} = \sqrt[72]{1}\\
        \omega_k = \cos{\frac{2k\pi}{72}} + \imath\sin{\frac{2k\pi}{72}}\\
        \omega_0 ^ {389} + \omega_1 ^ {389} + \dots + \omega_{71} ^ {389} = ?\\
        \omega_0 ^ {389} + \omega_1 ^ {389} + \dots + \omega_{71} ^ {389} = \displaystyle\sum_{i=0}^{71} \omega_i ^ {389}\\
        \omega_1 \in \mathbb{C}\\
        \implies \omega_1 ^ k = \cos{\frac{2k\pi}{72}} + \imath\sin{\frac{2k\pi}{72}} = \omega_k\\
        \implies \displaystyle\sum_{i=0}^{71} \omega_i ^ {389}
        = \displaystyle\sum_{i=0}^{71} \left(\omega_1 ^ {389}\right) ^ i
        = \frac{\left(\omega_1 ^ {389}\right) ^ {72} - 1}{\omega_1 ^ {389} - 1}\\
        = \frac{\left(\cos{\frac{2\times\stkout{72}\times389\pi}{\stkout{72}}} + \imath\sin{\frac{2\times\stkout{72}\times389\pi}{\stkout{72}}}\right) - 1}{\omega_1 ^ {389} - 1}\\
        = \frac{\left(\cos{2\times389\pi} + \imath\sin{2\times389\pi}\right) - 1}{\omega_1 ^ {389} - 1}\\
        = \frac{\left(\cos\pi + \imath\sin\pi\right) - 1}{\omega_1 ^ {389} - 1} = \frac{1 + 0\imath - 1}{\omega_1 ^ {389} - 1} = \frac{0}{\omega_1 ^ {389} - 1}\\
        \omega_1 ^ {389} = \cos{\frac{2\pi389}{72}} + \imath\sin{\frac{2\pi389}{72}} \neq 1\\
        \implies \omega_1 ^ {389} - 1 \neq 0\\
        \implies \frac{0}{\omega_1 ^ {389} - 1} = 0\\
        \implies \omega_0 ^ {389} + \omega_1 ^ {389} + \dots + \omega_{71} ^ {389} = 0
    \end{align*}
\end{document}`