\documentclass{article}
\usepackage{amsmath}
\usepackage{amssymb}
\usepackage[T1,T2A]{fontenc}
\usepackage[utf8]{inputenc}
\usepackage[bulgarian]{babel}
\usepackage[normalem]{ulem}
\newcommand{\stkout}[1]{\ifmmode\text{\sout{\ensuremath{#1}}}\else\sout{#1}\fi}

\makeatletter
\renewcommand*\env@matrix[1][*\c@MaxMatrixCols c]{%
  \hskip -\arraycolsep
  \let\@ifnextchar\new@ifnextchar
  \array{#1}}
\makeatother

\begin{document}
    \pagenumbering{gobble}
    \begin{math}
        \begin{array}{rcl}
            v_1 & = & (-4, 3, 5, -3)\\
            v_2 & = & (-4, -1, 8, -14)\\
            v_3 & = & (-1, 1, 1, 0)\\
            v_4 & = & (-1, -3, 2,\mu - 8)\\
            v & = & (1, 1, \lambda, 1)
        \end{array}\\
        \\
        \\
        \begin{matrix}
          ~\\
          1\\
          1\\
          ~
        \end{matrix}
        \begin{pmatrix}[cccc|c]
             -4 & -4 & -1 & -1 & 1\\
             3 & -1 & 1 & -3 & 1\\
             5 & 8 & 1 & 2 & \lambda\\
             -3 & -14 & 0 & \mu - 8 & 1
        \end{pmatrix}\\
        \\
        \\
        \to
        \begin{matrix}
          -4\\
          ~\\
          1\\
          -3
        \end{matrix}
        \begin{pmatrix}[cccc|c]
             -4 & -4 & -1 & -1 & 1\\
             -1 & -5 & 0 & -4 & 2\\
             1 & 4 & 0 & 1 & \lambda + 1\\
             -3 & -14 & 0 & \mu - 8 & 1
        \end{pmatrix}
        \\
        \\
        \\
        \to
        \begin{matrix}
          16\\
          -5\\
          ~\\
          1
        \end{matrix}
        \begin{pmatrix}[cccc|c]
             0 & 16 & -1 & 15 & -7\\
             -1 & -5 & 0 & -4 & 2\\
             0 & -1 & 0 & -3 & \lambda + 3\\
             0 & 1 & 0 & \mu + 4 & -5
        \end{pmatrix}\\
        \\
        \\
        \to
        \begin{pmatrix}[cccc|c]
             0 & 0 & -1 & -33 & 16\lambda + 41\\
             -1 & 0 & 0 & 11 & -5\lambda - 13\\
             0 & -1 & 0 & -3 & \lambda + 3\\
             0 & 0 & 0 & \mu + 1 & \lambda - 2
        \end{pmatrix}
        \begin{matrix}
          -1\\
          -1\\
          -1\\
          ~
        \end{matrix}
        \\
        \\
        \\
        \begin{matrix}[|ccccc]
            x_3 & + & 33x_4 & = & -16\lambda - 41\\
            x_1 & + & -11x_4 & = & 5\lambda + 13\\
            x_2 & + & 3x_4 & = & -\lambda - 3\\
            ~ & ~ & (\mu + 1)x_4 & = & \lambda - 2\\
        \end{matrix}
    \end{math}
    \section{\(\mu = -1\)}
    \subsection{\(\lambda = 2\)}
    \begin{math}
       \begin{matrix}[|ccccc]
            x_3 & + & 33x_4 & = & -16\lambda - 41\\
            x_1 & + & -11x_4 & = & 5\lambda + 13\\
            x_2 & + & 3x_4 & = & -\lambda - 3\\
            ~ & ~ & 0x_4 & = & 0\\
        \end{matrix}\\
        \\
        \\
        \to\quad
        \begin{matrix}[|ccccc]
            x_3 & + & 33x_4 & = & -16\lambda - 41\\
            x_1 & + & -11x_4 & = & 5\lambda + 13\\
            x_2 & + & 3x_4 & = & -\lambda - 3\\
        \end{matrix}\\
        \\
        x_4 = p\\
        \\
        \begin{matrix}[|ccccc]
            x_3 & + & 33p & = & -16\lambda - 41\\
            x_1 & + & -11p & = & 5\lambda + 13\\
            x_2 & + & 3p & = & -\lambda - 3\\
        \end{matrix}\\
        \\
        \\
        \to\quad
        \begin{matrix}[|ccc]
            x_3 & = & -16\lambda - 41 - 33p\\
            x_1 & = & 5\lambda + 13 + 11p\\
            x_2 & = & -\lambda - 3 - 3p\\
        \end{matrix}
    \end{math}
    \subsection{\(\lambda \neq 2\)}
    \begin{math}
       \begin{matrix}[|ccccc]
            x_3 & + & 33x_4 & = & -16\lambda - 41\\
            x_1 & + & -11x_4 & = & 5\lambda + 13\\
            x_2 & + & 3x_4 & = & -\lambda - 3\\
            ~ & ~ & 0x_4 & = & \lambda - 2\\
        \end{matrix}
    \end{math}
    \section{\(\mu \neq -1\)}
    \subsection{\(\lambda = 2\)}
    \begin{math}
       \begin{matrix}[|ccccc]
            x_3 & + & 33x_4 & = & -16\lambda - 41\\
            x_1 & + & -11x_4 & = & 5\lambda + 13\\
            x_2 & + & 3x_4 & = & -\lambda - 3\\
            ~ & ~ & (\mu + 1)x_4 & = & 0\\
        \end{matrix}\\
        \\
        \\
        \to\quad
        \begin{matrix}[|ccc]
            x_3 & = & -16\lambda - 41\\
            x_1 & = & 5\lambda + 13\\
            x_2 & = & -\lambda - 3\\
            x_4 & = & 0\\
        \end{matrix}\\
    \end{math}
    \subsection{\(\lambda \neq 2\)}
    \begin{math}
       \begin{matrix}[|ccccc]
            x_3 & + & 33x_4 & = & -16\lambda - 41\\
            x_1 & + & -11x_4 & = & 5\lambda + 13\\
            x_2 & + & 3x_4 & = & -\lambda - 3\\
            ~ & ~ & (\mu + 1)x_4 & = & \lambda - 2\\
        \end{matrix}\\
        \\
        \\
        \to\quad
        \begin{matrix}[|ccc]
            x_3 & = & \frac{-(16\lambda + 41)(\mu + 1) - 33(\lambda - 2)}{\mu + 1}\\
            x_1 & = & \frac{(5\lambda + 13)(\mu + 1) + 11(\lambda - 2)}{\mu + 1}\\
            x_2 & = & \frac{-(\lambda + 3)(\mu + 1) - 3(\lambda - 2)}{\mu + 1}\\
            x_4 & = & \frac{\lambda - 2}{\mu + 1}
        \end{matrix}\\
        \\
        \\
        \to\quad
        \begin{matrix}[|ccc]
            x_3 & = & \frac{-(16\lambda\mu + 40\lambda + 41\mu - 25)}{\mu + 1}\\
            x_1 & = & \frac{5\lambda\mu + 16\lambda + 13\mu - 9}{\mu + 1}\\
            x_2 & = & \frac{-(\lambda\mu + 4\lambda + 3\mu -3)}{\mu + 1}\\
            x_4 & = & \frac{\lambda - 2}{\mu + 1}
        \end{matrix}
    \end{math}
\end{document}