\documentclass{article}
\usepackage{amsmath}
\usepackage{amssymb}
\usepackage[T1,T2A]{fontenc}
\usepackage[utf8]{inputenc}
\usepackage[bulgarian]{babel}
\usepackage[normalem]{ulem}
\newcommand{\stkout}[1]{\ifmmode\text{\sout{\ensuremath{#1}}}\else\sout{#1}\fi}

\begin{document}
    \pagenumbering{gobble}
    \begin{math}
        \\
        (x - \imath) ^ {36} + (x + \imath) ^ {36} = 0\\
        (x - \imath) ^ {36} = -(x + \imath) ^ {36}\\
        x \neq \imath\\
        \left(\frac{x - \imath}{x + \imath}\right) ^ {36} = -1\\
        A = \frac{x - \imath}{x + \imath}\\
        A ^ {36} = -1\\
        z = -1 = -1 + 0\imath\\
        |z| = \sqrt{1} = 1\\
        \cos\varphi = \frac{-1}{1} = -1, \sin\varphi = \frac{0}{1} = 0 \implies \varphi = \pi\\
        z = \cos\pi + \imath\sin\pi\\
        \sqrt[36]z = \cos{\frac{\pi + 2k\pi}{36}} + \imath\sin{\frac{\pi + 2k\pi}{36}} = z_k\\
        k = 0, 1, \dots, 35\\
        \frac{x - \imath}{x + \imath} = z_k\\
        x - \imath = z_k(x + \imath)\\
        x - \imath = z_kx + z_k\imath\\
        \imath - z_k\imath = z_kx + x\\
        (1 - z_k)\imath = (z_k + 1)x\\
        z_k < \cos{\frac{\pi + 2\pi\stkout{36}}{\stkout{36}}} + \imath\sin{\frac{\pi + 2\pi\stkout{36}}{\stkout{36}}} = \cos\pi + \imath\sin\pi = -1\\
        \implies z_k + 1 \neq 0\\
        x = \frac{(z_k - 1)\imath}{(z_k + 1)}
    \end{math}
\end{document}
